AwsCryptographicMaterialProviders/dafny/AwsCryptographyKeyStore/test/TestGetKeys.dfy
@@ -12,6 +12,8 @@ module TestGetKeys {
   import opened Wrappers
 
   const branchKeyStoreName := "KeyStoreTestTable";
+  const logicalKeyStoreName := branchKeyStoreName;
+  const incorrectLogicalName := "MySuperAwesomeTableName";
   const branchKeyId := "71c83ce3-aad6-4aab-a4c4-d02bb9273305";
   // THESE ARE TESTING RESOURCES DO NOT USE IN A PRODUCTION ENVIRONMENT
   const keyArn := "arn:aws:kms:us-west-2:370957321024:key/9d989aa2-2f9c-438c-a745-cc57d3ad0126";
@@ -21,9 +23,12 @@ module TestGetKeys {
   {
     var kmsClient :- expect KMS.KMSClient();
     var ddbClient :- expect DDB.DynamoDBClient();
+    var kmsConfig := Types.KMSConfiguration.kmsKeyArn(keyArn);
+
     var keyStoreConfig := Types.KeyStoreConfig(
       id := None,
-      kmsKeyArn := keyArn,
+      kmsConfiguration := kmsConfig,
+      logicalKeyStoreName := logicalKeyStoreName,
       grantTokens := None,
       ddbTableName := branchKeyStoreName,
       ddbClient := Some(ddbClient),
@@ -42,9 +47,12 @@ module TestGetKeys {
   {
     var kmsClient :- expect KMS.KMSClient();
     var ddbClient :- expect DDB.DynamoDBClient();
+    var kmsConfig := Types.KMSConfiguration.kmsKeyArn(keyArn);
+
     var keyStoreConfig := Types.KeyStoreConfig(
       id := None,
-      kmsKeyArn := keyArn,
+      kmsConfiguration := kmsConfig,
+      logicalKeyStoreName := logicalKeyStoreName,
       grantTokens := None,
       ddbTableName := branchKeyStoreName,
       ddbClient := Some(ddbClient),
@@ -63,9 +71,12 @@ module TestGetKeys {
   method {:test} TestGetActiveKeyWithIncorrectKmsKeyArn() {
     var kmsClient :- expect KMS.KMSClient();
     var ddbClient :- expect DDB.DynamoDBClient();
+    var kmsConfig := Types.KMSConfiguration.kmsKeyArn(mkrKeyArn);
+
     var keyStoreConfig := Types.KeyStoreConfig(
       id := None,
-      kmsKeyArn := mkrKeyArn,
+      kmsConfiguration := kmsConfig,
+      logicalKeyStoreName := logicalKeyStoreName,
       grantTokens := None,
       ddbTableName := branchKeyStoreName,
       ddbClient := Some(ddbClient),
@@ -80,6 +91,52 @@ module TestGetKeys {
 
     expect activeResult.Failure?;
     expect activeResult.error == Types.KeyStoreException(
-      message :="Configured AWS KMS Key ARN does not match KMS Key ARN for branch-key-id: " + branchKeyId);
+      message := "Configured AWS KMS Key ARN does not match KMS Key ARN for branch-key-id: " + branchKeyId);
+  }
+
+  method {:test} TestGetActiveKeyWrongLogicalKeyStoreName() {
+    var kmsClient :- expect KMS.KMSClient();
+    var ddbClient :- expect DDB.DynamoDBClient();
+    var kmsConfig := Types.KMSConfiguration.kmsKeyArn(keyArn);
+
+    var keyStoreConfig := Types.KeyStoreConfig(
+      id := None,
+      kmsConfiguration := kmsConfig,
+      logicalKeyStoreName := incorrectLogicalName,
+      grantTokens := None,
+      ddbTableName := branchKeyStoreName,
+      ddbClient := Some(ddbClient),
+      kmsClient := Some(kmsClient)
+    );
+
+    var keyStore :- expect KeyStore.KeyStore(keyStoreConfig);
+
+    var activeResult := keyStore.GetActiveBranchKey(Types.GetActiveBranchKeyInput(
+      branchKeyIdentifier := branchKeyId
+    ));
+
+    expect activeResult.Failure?;
+  }
+
+  method {:test} TestGetActiveKeyWithNoClients() {
+    var kmsConfig := Types.KMSConfiguration.kmsKeyArn(keyArn);
+
+    var keyStoreConfig := Types.KeyStoreConfig(
+      id := None,
+      kmsConfiguration := kmsConfig,
+      logicalKeyStoreName := logicalKeyStoreName,
+      grantTokens := None,
+      ddbTableName := branchKeyStoreName,
+      ddbClient := None,
+      kmsClient := None
+    );
+
+    var keyStore :- expect KeyStore.KeyStore(keyStoreConfig);
+
+    var activeResult :- expect keyStore.GetActiveBranchKey(Types.GetActiveBranchKeyInput(
+      branchKeyIdentifier := branchKeyId
+    ));
+    
+    expect |activeResult.branchKey| == 32;
   }
 }
