AwsCryptographicMaterialProviders/dafny/AwsCryptographyKeyStore/test/TestKeyResolution.dfy
@@ -22,15 +22,19 @@ module TestKeyResolution {
   import opened KeyResolution
   
   const branchKeyStoreName := "KeyStoreTestTable";
+  const logicalKeyStoreName := branchKeyStoreName;
   // THESE ARE TESTING RESOURCES DO NOT USE IN A PRODUCTION ENVIRONMENT
   const keyArn := "arn:aws:kms:us-west-2:370957321024:key/9d989aa2-2f9c-438c-a745-cc57d3ad0126";
 
   method {:test} TestActiveBranchKeyResolution() {
     var kmsClient :- expect KMS.KMSClient();
     var ddbClient :- expect DDB.DynamoDBClient();
+    var kmsConfig := Types.KMSConfiguration.kmsKeyArn(keyArn);
+    
     var keyStoreConfig := Types.KeyStoreConfig(
       id := None,
-      kmsKeyArn := keyArn,
+      kmsConfiguration := kmsConfig,
+      logicalKeyStoreName := logicalKeyStoreName,
       grantTokens := None,
       ddbTableName := branchKeyStoreName,
       ddbClient := Some(ddbClient),
@@ -74,7 +78,7 @@ module TestKeyResolution {
       branchKeyIdentifer,
       version.value,
       timestamp.value,
-      branchKeyStoreName,
+      logicalKeyStoreName,
       keyArn
     );
 
